src/util/Word.v
@@ -1,0 +1,393 @@
+Require Import Coq.ZArith.ZArith.
+Require Import Coq.Logic.ProofIrrelevance.
+Require Import bbv.ZLib.
+Require Import riscv.util.ZBitOps.
+Require Import riscv.util.Tactics.
+Require Import riscv.util.div_mod_to_quot_rem.
+Local Open Scope Z_scope.
+
+
+Definition word(sz: Z) := { x: Z | x mod 2 ^ sz = x }.
+
+Definition ZToWord(sz: Z)(x: Z): word sz := 
+  exist _ (x mod 2 ^ sz) (Zmod_mod x (2 ^ sz)).
+
+Definition uwordToZ{sz: Z}: word sz -> Z := @proj1_sig Z (fun x => x mod 2 ^ sz = x).
+
+Definition wmsb{sz: Z}(a: word sz): bool := Z.testbit (uwordToZ a) (sz - 1).
+
+Definition swordToZ{sz: Z}(a: word sz): Z :=
+  if wmsb a then uwordToZ a - 2 ^ sz else uwordToZ a.
+
+Definition wu_unop(f: Z -> Z)(sz: Z)(a: word sz): word sz :=
+  ZToWord sz (f (uwordToZ a)).
+
+Definition wu_binop(f: Z -> Z -> Z)(sz: Z)(a b: word sz): word sz :=
+  ZToWord sz (f (uwordToZ a) (uwordToZ b)).
+
+Definition wu_binop_t{T: Type}(f: Z -> Z -> T)(sz: Z)(a b: word sz): T :=
+  f (uwordToZ a) (uwordToZ b).
+
+Definition ws_unop(f: Z -> Z)(sz: Z)(a: word sz): word sz :=
+  ZToWord sz (f (swordToZ a)).
+
+Definition ws_binop(f: Z -> Z -> Z)(sz: Z)(a b: word sz): word sz :=
+  ZToWord sz (f (swordToZ a) (swordToZ b)).
+
+Definition ws_binop_t{T: Type}(f: Z -> Z -> T)(sz: Z)(a b: word sz): T :=
+  f (swordToZ a) (swordToZ b).
+
+Hint Unfold ZToWord uwordToZ wmsb swordToZ
+            wu_unop wu_binop wu_binop_t
+            ws_unop ws_binop ws_binop_t
+            proj1_sig
+: unf_word_all.
+
+
+Section ArithOps.
+
+  Context {sz: Z}.
+
+  Definition wopp := ws_unop Z.opp sz.
+
+  Definition wadd := wu_binop Z.add sz.
+  Definition wsub := wu_binop Z.sub sz.
+  Definition wmul := wu_binop Z.mul sz.
+
+  Definition wsadd := ws_binop Z.add sz.
+  Definition wssub := ws_binop Z.sub sz.
+  Definition wsmul := ws_binop Z.mul sz.
+
+End ArithOps.
+
+Hint Unfold wopp wadd wsub wmul wsadd wssub wsmul : unf_word_all.
+
+
+Ltac make_mod_nonzero :=
+  let C := fresh in
+  match goal with
+  | |- context [_ mod ?m] =>
+    assert (m = 0 \/ m <> 0) as C by omega;
+    destruct C as [C | C];
+    [ rewrite C in *; rewrite? Zmod_0_r; reflexivity | ]
+  end.
+
+Ltac mod0_exists_quotient H :=
+  apply Z.mod_divide in H;
+  [ let k := fresh "k" in let E := fresh "E" in unfold Z.divide in H; destruct H as [k E] | ].  
+
+Lemma mod_eq_from_diff: forall a b m,
+    (a - b) mod m = 0 ->
+    a mod m = b mod m.
+Proof.
+  intros.
+  make_mod_nonzero.
+  mod0_exists_quotient H; [|assumption].
+  replace a with (b + k * m) by omega.
+  apply Z_mod_plus_full.
+Qed.
+
+Lemma mod_eq_to_diff: forall a b m : Z,
+    a mod m = b mod m ->
+    (a - b) mod m = 0.
+Proof.
+  intros.
+  make_mod_nonzero.
+  apply Z.mod_divide; [assumption|].
+  unfold Z.divide.
+  div_mod_to_quot_rem.
+  subst a b r0.
+  exists (q - q0).
+  ring.
+Qed.
+
+Ltac prove_mod_0 :=
+  match goal with
+  | |- ?a mod ?m = 0 => ring_simplify a
+  end;
+  rewrite? Zplus_mod_idemp_l;
+  rewrite? Zplus_mod_idemp_r;
+  rewrite? Zminus_mod_idemp_l;
+  rewrite? Zminus_mod_idemp_r;
+  rewrite? Zmult_mod_idemp_l;
+  rewrite? Zmult_mod_idemp_r;
+  match goal with
+  | |- ?a mod ?m = 0 => ring_simplify a
+  end;
+  rewrite? Z.pow_2_r;
+  first
+    (* base cases: *)
+    [ apply Z_mod_mult
+    | apply Z_mod_mult'
+    | apply Z_mod_same_full
+    | apply Zmod_0_l
+    (* cases with recursion (the last two might turn a true goal into a false one): *)
+    | apply Z_mod_zero_opp_full
+    | apply add_mod_0
+    | apply sub_mod_0
+ (* | match goal with
+      | |- ?G => fail 1000 "failed to solve" G
+      end *)
+    ];
+  [> prove_mod_0 .. ].
+
+Ltac word_destruct :=
+  intuition idtac;
+  repeat autounfold with unf_word_all in *;
+  repeat match goal with
+         | w: word _ |- _ => let H := fresh "M" w in destruct w as [w H]
+         end;
+  repeat match goal with
+         | H: (?x =? ?y) = true |- _ =>
+           apply Z.eqb_eq in H; try subst x; try subst y
+         | H: exist _ ?x _ = exist _ ?y _ |- _ =>
+           apply EqdepFacts.eq_sig_fst in H; try subst x; try subst y
+  end;
+  repeat match goal with
+         | |- context[if ?b then _ else _] => let E := fresh "E" in destruct b eqn: E
+         end.
+
+Ltac word_eq_pre :=
+  repeat match goal with
+         | H: ?a mod ?m = ?b mod ?m |- _ =>
+           apply mod_eq_to_diff in H;
+           match type of H with
+           | ?a mod ?m = 0 => ring_simplify a in H
+           end
+         end;
+  try apply subset_eq_compat;
+  try apply Z.eqb_refl;
+  auto;
+  try match goal with
+      | H: ?b mod ?m = ?b |- _  = ?b => refine (eq_trans _ H)
+      end;
+  try match goal with
+      | H: ?a mod ?m = ?a |- ?a = _  => refine (eq_trans (eq_sym H) _)
+      end;
+  rewrite? Zplus_mod_idemp_l;
+  rewrite? Zplus_mod_idemp_r;
+  rewrite? Zminus_mod_idemp_l;
+  rewrite? Zminus_mod_idemp_r;
+  rewrite? Zmult_mod_idemp_l;
+  rewrite? Zmult_mod_idemp_r;
+  apply mod_eq_from_diff.
+
+Ltac word_solver := word_destruct; word_eq_pre; prove_mod_0.
+
+
+Section ArithOpsEquiv.
+
+  Context {sz: Z}.
+
+  Lemma wadd_wsadd: forall a b: word sz,
+      wadd a b = wsadd a b.
+  Proof. word_solver. Qed.
+
+  Lemma wsub_wssub: forall a b: word sz,
+      wsub a b = wssub a b.
+  Proof. word_solver. Qed.
+
+  Lemma wmul_wsmul: forall a b: word sz,
+      wmul a b = wsmul a b.
+  Proof. word_solver. Qed.
+
+End ArithOpsEquiv.
+
+
+Section MoreOps.
+
+  Context {sz: Z}.
+
+  Definition wudiv  := wu_binop Z.div sz.
+  Definition wuquot := wu_binop Z.quot sz.
+  Definition wumod  := wu_binop Z.modulo sz.
+  Definition wurem  := wu_binop Z.rem sz.
+
+  Definition wsdiv  := ws_binop Z.div sz.
+  Definition wsquot := ws_binop Z.quot sz.
+  Definition wsmod  := ws_binop Z.modulo sz.
+  Definition wsrem  := ws_binop Z.rem sz.
+  
+  Definition wor   := wu_binop Z.lor sz.
+  Definition wand  := wu_binop Z.land sz.
+  Definition wxor  := wu_binop Z.lxor sz.
+
+  Definition weqb := wu_binop_t Z.eqb sz.
+
+  Definition wuleb := wu_binop_t Z.leb sz.
+  Definition wultb := wu_binop_t Z.ltb sz.
+  Definition wugeb := wu_binop_t Z.geb sz.
+  Definition wugtb := wu_binop_t Z.gtb sz.
+
+  Definition wsleb := ws_binop_t Z.leb sz.
+  Definition wsltb := ws_binop_t Z.ltb sz.
+  Definition wsgeb := ws_binop_t Z.geb sz.
+  Definition wsgtb := ws_binop_t Z.gtb sz.
+
+  Definition wshiftl  := wu_binop Z.shiftl sz.
+  Definition wshiftr  := wu_binop Z.shiftr sz.
+  Definition wshiftra := ws_binop Z.shiftr sz.
+
+End MoreOps.
+
+Hint Unfold
+    wudiv wuquot wumod wurem
+    wsdiv wsquot wsmod wsrem
+    wor wand wxor
+    weqb
+    wuleb wultb wugeb wugtb
+    wsleb wsltb wsgeb wsgtb
+    wshiftl wshiftr wshiftra
+: unf_word_all.
+
+
+Definition wucast{sz: Z}(sz': Z)(w: word sz): word sz' :=
+  ZToWord sz' (uwordToZ w).
+
+Definition wscast{sz: Z}(sz': Z)(w: word sz): word sz' :=
+  ZToWord sz' (swordToZ w).
+
+(*
+Definition wappend{sz1 sz2: Z}(w1: word sz1)(w2: word sz2): word (sz1 + sz2) :=
+  ZToWord (sz1 + sz2) (2 ^ sz2 * (uwordToZ w1) + uwordToZ w2).
+*)
+Definition wappend{sz1 sz2: Z}(w1: word sz1)(w2: word sz2): word (sz1 + sz2) :=
+  ZToWord (sz1 + sz2) (Z.lor (2 ^ sz2 * (uwordToZ w1)) (uwordToZ w2)).
+
+(*
+Definition wslice{sz: Z}(w: word sz)(i j: Z): word (j - i) :=
+  ZToWord (j - i) (bitSlice (uwordToZ w) i j).
+
+Definition lobits(sz: Z)(w: word (2 * sz)): word sz.
+  wslice w sz (2 * sz).
+
+Definition hibits(sz: Z)(w: word (2 * sz)): word sz :=
+  ZToWord sz (bitSlice (uwordToZ w) sz (2 * sz)).
+
+Definition wslice(sz1 sz2 sz3: Z)(w: word (sz1 + sz2 + sz3)): word sz2 :=
+  ZToWord sz2 (bitSlice (uwordToZ w) sz1 (sz1 + sz2)).
+ *)
+
+Definition wsplit_lo(sz1 sz2: Z)(w: word (sz1 + sz2)): word sz2 :=
+  wucast sz2 w.
+
+Definition wsplit_hi(sz1 sz2: Z)(w: word (sz1 + sz2)): word sz1 :=
+  ZToWord sz1 (Z.shiftr (uwordToZ w) sz2).
+
+Definition lobits(sz: Z)(w: word (sz + sz)): word sz := wsplit_lo sz sz w.
+
+Definition hibits(sz: Z)(w: word (sz + sz)): word sz := wsplit_hi sz sz w.
+
+Hint Unfold wucast wscast wappend wsplit_lo wsplit_hi lobits hibits : unf_word_all.
+
+Ltac word_omega_pre :=
+      repeat match goal with
+         | n: Z |- _ => 
+           let B := fresh in assert (0 < n) by omega;
+           unique pose proof (pow2_times2 n B)
+         | _: context[2 ^ ?n] |- _ =>
+           let B := fresh in assert (0 <= n) by omega;
+           unique pose proof (pow2_pos n B)
+         | _: context[?a mod ?m] |- _ =>
+           let B := fresh in assert (0 < m) by omega;
+           unique pose proof (Z.mod_pos_bound a m B)
+         | H: ?a mod 2 ^ _ = ?a      |- _ => apply mod_pow2_same_bounds in H; [|omega]
+         | H: Z.testbit _ _ = true   |- _ => apply testbit_true_nonneg in H; [|omega..]
+         | H: Z.testbit _ _ = false  |- _ => apply testbit_false_nonneg in H; [|omega..]
+         | H1: ?a <= ?b, H2: ?b < ?c  |- _ => unique pose proof (conj H1 H2)
+         | H: - 2 ^ _ <= ?n < 2 ^ _   |- _ => unique pose proof (signed_bounds_to_sz_pos _ _ H)
+         end.
+
+Ltac word_omega := word_omega_pre; omega.
+
+Lemma wappend_split: forall sz1 sz2 (w : word (sz1 + sz2)),
+    wappend (wsplit_hi sz1 sz2 w) (wsplit_lo sz1 sz2 w) = w.
+Proof.
+Admitted.
+
+Lemma wappend_inj: forall sz1 sz2 (a : word sz1) (b : word sz2) (c : word sz1) (d : word sz2),
+    0 <= sz1 ->
+    0 <= sz2 ->
+    wappend a b = wappend c d ->
+    a = c /\ b = d.
+Proof.
+  word_destruct; word_eq_pre.
+  - mod0_exists_quotient H1; [|word_omega].
+    replace (2 ^ sz2 * a - 2 ^ sz2 * c + b - d) with
+            (b - d + (a - c) * (2 ^ sz2)) in E by ring.
+    rewrite Z.pow_add_r in E by omega.
+Admitted.
+
+Lemma word_ring: forall sz,
+    ring_theory (ZToWord sz 0) (ZToWord sz 1) wadd wmul wsub wopp eq.
+Proof.
+  intros. constructor; word_solver.
+Qed.
+
+Lemma word_ring_morph_Z: forall sz,
+    ring_morph (ZToWord sz 0) (ZToWord sz 1) wadd  wmul  wsub  wopp  eq
+               0              1              Z.add Z.mul Z.sub Z.opp Z.eqb
+               (ZToWord sz).
+Proof.
+  intros. constructor; word_solver.
+Qed.
+
+Lemma weqb_spec: forall sz (a b : word sz),
+    weqb a b = true <-> a = b.
+Proof. word_solver. Qed.
+
+Lemma swordToZ_bound: forall sz (a : word sz),
+    0 < sz ->
+    - 2 ^ (sz - 1) <= swordToZ a < 2 ^ (sz - 1).
+Proof. word_destruct; word_omega. Qed.
+
+Lemma uwordToZ_bound: forall sz (a : word sz),
+    0 < sz ->
+    0 <= uwordToZ a < 2 ^ sz.
+Proof. word_destruct; word_omega. Qed.
+
+Lemma swordToZ_ZToWord: forall sz n,
+    - 2 ^ (sz - 1) <= n < 2 ^ (sz - 1) ->
+    swordToZ (ZToWord sz n) = n.
+Proof.
+  word_destruct; word_omega_pre;
+    assert (sz = 1 \/ 1 < sz) as C by omega;
+    (destruct C as [C | C];
+     [subst sz;
+      repeat match goal with
+             | _: context[2 ^ ?x] |- _ =>
+               let r := eval cbv in (2 ^ x) in change (2 ^ x) with r in *
+             end;
+      assert (n = -1 \/ n = 0) as C by omega;
+      destruct C; subst n; cbv in E; try reflexivity; congruence |]);
+      match goal with
+        | _: context[?a mod ?m] |- _ =>
+          let B := fresh in
+          assert (m <> 0) by omega;
+          pose proof (Z.mod_eq a m B) as M
+        end;
+      assert (- 2 ^ (sz - 1) <= n <= 2 ^ (sz - 1) + 1) as B by omega;
+      (apply (range_div_pos _ _ _ (2 ^ sz)) in B; [|omega]);
+      assert (2 ^ (sz - 1) mod 2 ^ sz = 2 ^ (sz - 1)) by (apply Z.mod_small; omega);
+      rewrite Z.div_opp_l_nz in B by omega;
+      rewrite Z.div_small in B by omega;
+      (rewrite (Z.div_small (2 ^ (sz - 1) + 1) (2 ^ sz)) in B;
+       [ assert (n / 2 ^ sz = 0 \/ n / 2 ^ sz = -1) as R by omega;
+         destruct R as [R | R]; rewrite R in M; omega
+       | split; try omega;
+         rewrite H4;
+         pose proof (Z.pow_gt_1 2 (sz - 1));
+         omega ]).
+Qed.
+
+Lemma uwordToZ_ZToWord_mod: forall sz n,
+    uwordToZ (ZToWord sz n) = n mod 2 ^ sz.
+Proof. intros. reflexivity. Qed.
+
+Lemma ZToWord_uwordToZ: forall sz (a : word sz),
+    ZToWord sz (uwordToZ a) = a.
+Proof. word_solver. Qed.
+
+Lemma ZToWord_swordToZ: forall sz (a : word sz),
+    ZToWord sz (swordToZ a) = a.
+Proof. word_solver. Qed.
